processors/DMem.v
@@ -1,0 +1,72 @@
+Require Import Kami.
+Require Import Lib.Indexer.
+Require Import Ex.MemTypes Ex.OneEltFifo.
+Require Import Mem AbstractIsa.
+
+Set Implicit Arguments.
+
+Section DMem.
+  Variables addrSize dataBytes rfIdx: nat.
+  Variables (m2dName d2wName dExecName: string).
+
+  Definition M2D := M2D addrSize dataBytes rfIdx.
+
+  Definition D2W :=
+    STRUCT { "m2wOrig" :: Struct (M2W addrSize dataBytes rfIdx);
+             "dMemRep" :: Struct (RsToProc dataBytes) }.
+
+  Definition m2dDeq := MethodSig (m2dName -- "deq")(): Struct M2D.
+  Definition d2wEnq := MethodSig (d2wName -- "enq")(Struct D2W): Void.
+
+  Definition exec :=
+    MethodSig dExecName(Struct (RqFromProc dataBytes (Bit addrSize))) : Struct (RsToProc dataBytes).
+
+  Definition dMem :=
+    MODULE {
+      Rule "passDMem" :=
+        Call m2d <- m2dDeq();
+        LET m2wOrig <- #m2d!M2D@."m2wOrig";
+        Assert (#m2wOrig!(M2W addrSize dataBytes rfIdx)@."poisoned");
+        Call d2wEnq(STRUCT { "m2wOrig" ::= #m2wOrig;
+                             "dMemRep" ::= $$Default });
+        Retv
+     
+      with Rule "doDMem" :=
+        Call m2d <- m2dDeq();
+        LET m2wOrig <- #m2d!M2D@."m2wOrig";
+        Assert (!#m2wOrig!(M2W addrSize dataBytes rfIdx)@."poisoned");
+
+        LET eInst <- #m2wOrig!(M2W addrSize dataBytes rfIdx)@."eInst";
+        LET iType <- #eInst!(execInst addrSize dataBytes rfIdx)@."iType";
+
+        If (#iType == $$iTypeLd || #iType == $$iTypeSt)
+        then
+          LET req <- #m2d!M2D@."dMemReq";
+          Call rep <- exec(#req);
+          Call d2wEnq (STRUCT { "m2wOrig" ::= #m2wOrig;
+                                "dMemRep" ::= #rep });
+          Retv
+        else
+          Call d2wEnq(STRUCT { "m2wOrig" ::= #m2wOrig;
+                               "dMemRep" ::= $$Default });
+          Retv;
+        Retv
+      }.
+
+End DMem.
+
+Hint Unfold dMem : ModuleDefs.
+Hint Unfold M2D D2W m2dDeq d2wEnq exec : MethDefs.
+
+Section Wf.
+  Variables addrSize dataBytes rfIdx: nat.
+
+  Lemma dMem_ModEquiv:
+    forall m2dName d2wName dExecName,
+      ModPhoasWf (dMem addrSize dataBytes rfIdx m2dName d2wName dExecName).
+  Proof. kequiv. Qed.
+
+End Wf.
+
+Hint Resolve dMem_ModEquiv.
+                                            
