processors/IMem.v
@@ -1,0 +1,52 @@
+Require Import Kami.
+Require Import Lib.Indexer.
+Require Import Ex.MemTypes Ex.OneEltFifo.
+Require Import Fetch AbstractIsa.
+
+Set Implicit Arguments.
+
+Section IMem.
+  Variables addrSize dataBytes rfIdx: nat.
+  Variables (f2iName i2dName iExecName: string).
+
+  Definition F2I := F2I addrSize dataBytes.
+
+  Definition I2D :=
+    STRUCT { "f2dOrig" :: Struct (F2D addrSize);
+             "iMemRep" :: Struct (RsToProc dataBytes) }.
+
+  Definition f2iDeq := MethodSig (f2iName -- "deq")(): Struct F2I.
+  Definition i2dEnq := MethodSig (i2dName -- "enq")(Struct I2D): Void.
+
+  Definition exec :=
+    MethodSig iExecName(Struct (RqFromProc dataBytes (Bit addrSize))) : Struct (RsToProc dataBytes).
+
+  Definition iMem :=
+    MODULE {
+      Rule "doIMem" :=
+        Call f2i <- f2iDeq();
+        LET f2dOrig <- #f2i!F2I@."f2dOrig";
+        LET req <- #f2i!F2I@."iMemReq";
+        Call rep <- exec(#req);
+        Call i2dEnq(STRUCT { "f2dOrig" ::= #f2dOrig;
+                             "iMemRep" ::= #rep });
+        Retv
+    }.
+
+End IMem.
+
+Hint Unfold iMem : ModuleDefs.
+Hint Unfold F2I I2D f2iDeq i2dEnq exec : MethDefs.
+
+Section Wf.
+  Variables addrSize dataBytes rfIdx: nat.
+
+  Lemma iMem_ModEquiv:
+    forall f2iName i2dName iExecName,
+      ModPhoasWf (iMem addrSize dataBytes f2iName i2dName iExecName).
+  Proof. kequiv. Qed.
+
+End Wf.
+
+Hint Resolve iMem_ModEquiv.
+
