processors/Writeback.v
@@ -1,37 +1,60 @@
 Require Import Kami.
 Require Import Lib.Indexer.
 Require Import Ex.MemTypes Ex.OneEltFifo.
-Require Import AbstractIsa RegRead Mem Exception.
+Require Import AbstractIsa RegRead Mem DMem.
+
+(* NOTE: Let's add the exception mechanism after proving without it. *)
+(* Require Import Exception. *)
 
 Set Implicit Arguments.
 
 Section Processor.
   Variables addrSize dataBytes rfIdx: nat.
 
-  Section Writeback.
-    Variables (m2wName dMemRepName: string).
-    
-    Definition m2wDeq := MethodSig (m2wName -- "deq")(): Struct (M2W addrSize dataBytes rfIdx).
-    Definition dMemRep := MethodSig dMemRepName(): Struct (RsToProc dataBytes).
+  Section Csr.
+    Variable csrfIdx: nat.
 
-    (* TODO: implement *)
+    Definition csrfStr := STRUCT { "idx" :: Bit csrfIdx; "value" :: Data dataBytes }.
+
+    Definition csrfRd := MethodSig "csrfRd"(Bit csrfIdx) : Data dataBytes.
+    Definition csrfWr := MethodSig "csrfWr"(Struct csrfStr) : Void.
+
     Definition csrf :=
       MODULE {
-        Rule "dummy" := Retv
+        Register "csrf" : Vector (Data dataBytes) csrfIdx <- Default
+
+        with Method "csrfRd" (idx: Bit csrfIdx) : Data dataBytes :=
+          Read csrf <- "csrf";
+          Ret #csrf@[#idx]
+
+        with Method "csrfWr" (v: Struct csrfStr) : Void :=
+          Read csrf <- "csrf";
+          Write "csrf" <- #csrf@[#v!csrfStr@."idx" <- #v!csrfStr@."value"];
+          Retv
       }.
 
-    (* TODO: exception handling *)
+  End Csr.
+
+  Section Writeback.
+    Variable d2wName: string.
+    
+    Definition d2wDeq := MethodSig (d2wName -- "deq")(): Struct (D2W addrSize dataBytes rfIdx).
+
+    (* NOTE: handle exceptions later. *)
+    (* NOTE: handle CSRs later. *)
     
     Definition writeback :=
       MODULE {
         Rule "noWriteback" :=
-          Call m2w <- m2wDeq();
+          Call d2w <- d2wDeq();
           Call bpRemove();
-          Assert (#m2w!(M2W addrSize dataBytes rfIdx)@."poisoned");
+          LET m2wOrig <- #d2w!(D2W addrSize dataBytes rfIdx)@."m2wOrig";
+          Assert (#m2wOrig!(M2W addrSize dataBytes rfIdx)@."poisoned");
           Retv
 
         with Rule "doWriteback" :=
-          Call m2w <- m2wDeq();
+          Call d2w <- d2wDeq();
+          LET m2w <- #d2w!(D2W addrSize dataBytes rfIdx)@."m2wOrig";
           Call bpRemove();
           Assert (!#m2w!(M2W addrSize dataBytes rfIdx)@."poisoned");
 
@@ -41,7 +64,7 @@ Section Processor.
 
           If (#eInst!(execInst addrSize dataBytes rfIdx)@."iType" == $$iTypeLd)
           then
-            Call data <- dMemRep();
+            LET data <- #d2w!(D2W addrSize dataBytes rfIdx)@."dMemRep";
             Ret #data!(RsToProc dataBytes)@."data"
           else
             Ret (#eInst!(execInst addrSize dataBytes rfIdx)@."data")
