Makefile
@@ -1,13 +1,12 @@
 PROCVS:=$(wildcard processors/*.v)
-PROOFVS:=$(wildcard proofs/*.v)
 
 .PHONY: all clean
 
 all: Makefile.coq
 	$(MAKE) -f Makefile.coq
 
-Makefile.coq: Makefile $(PROCVS) $(PROOFVS)
-	coq_makefile -f _CoqProject $(PROCVS) $(PROOFVS) -o Makefile.coq
+Makefile.coq: Makefile $(PROCVS)
+	coq_makefile -f _CoqProject $(PROCVS) -o Makefile.coq
 
 clean:: Makefile.coq
 	$(MAKE) -f Makefile.coq clean
